defined bmatch and mmatch

rustfrontend/BorrowCheckSafe.v
@@ -1,16 +1,114 @@
-Require Import Coqlib.
-Require Import Errors.
+Require Import Coqlib .
+Require Import Errors Maps.
 Require Import Values.
+Require Import Integers.
 Require Import AST Errors.
 Require Import Memory.
 Require Import Events.
 Require Import Globalenvs.
-Require Import Smallstep SmallstepLinkingSafe.
+Require Import Smallstep SmallstepLinking SmallstepLinkingSafe.
 Require Import LanguageInterface Invariant.
-Require Import Rusttypes.
-Require Import RustIR BorrowCheckPolonius.
+Require Import Rusttypes RustlightBase.
+Require Import RustIR BorrowCheckDomain BorrowCheckPolonius.
 
-Section BORROWCK.
+(* move to rustlight  *)
+Definition is_owned (p: place) (own: own_env) : bool :=
+  match own ! (local_of_place p) with
+  | Some l =>
+      (** FIXME: consider partial ownership! *)
+      in_dec place_eq p l             
+  | None => false
+  end.
+
+Definition scalar_type (ty: type) : bool :=
+  match ty with
+  | Tunit
+  | Tint _ _
+  | Tlong _
+  | Tfloat _
+  | Tfunction _ _ _ _ _
+  | Tarray _ _ => true
+  | _ => false
+  end.
+
+(* relation between the selector and the (stmt, cont) pair *)
+Inductive match_instr_stmt (body: statement) : instruction -> statement -> cont -> Prop :=
+| sel_stmt_base: forall sel n s k,
+    select_stmt body sel = Some s ->
+    match_instr_stmt body (Isel sel n) s k
+| sel_stmt_seq: forall sel n s1 s2 k,
+    match_instr_stmt body (Isel sel n) s1 (Kseq s2 k) ->
+    match_instr_stmt body (Isel sel n) (Ssequence s1 s2) k
+| sel_stmt_kseq: forall sel n s k,
+    match_instr_stmt body (Isel sel n) s k ->
+    match_instr_stmt body (Isel sel n) Sskip (Kseq s k)
+| sel_stmt_ifthenelse: forall e n1 n2 s1 s2 k,
+    match_instr_stmt body (Icond e n1 n2) (Sifthenelse e s1 s2) k
+| sel_stmt_loop: forall n s k,    
+    match_instr_stmt body (Inop n) (Sloop s) k
+| sel_stmt_break: forall n k,    
+    match_instr_stmt body (Inop n) Sbreak k
+| sel_stmt_continue: forall n k,
+    match_instr_stmt body (Inop n) Scontinue k
+.
+
+(** Definition of abstracter which maps a memory location to place
+(i.e. the owner of this location) *)
+
+Definition mem_abstracter : Type := block -> Z -> option (place * Z).
+
+Section MATCH.
+
+Variable ce: composite_env.
+Variable abs: mem_abstracter.
+
+
+(* The value stored in m[b, ofs] is consistent with the type of p *)
+Inductive bmatch (m: mem) (b: block) (ofs: Z) (p: place) (own: own_env) : type -> Prop :=
+| bm_box: forall ty b1 ofs1
+    (* valid resource. If the loaded value is not a pointer, it is a
+    type error instead of a memory error *)
+    (VRES: Mem.load Mptr m b ofs = Some (Vptr b1 ofs1) ->
+           (abs b1 (Ptrofs.unsigned ofs1) = Some (Pderef p ty, 0) <-> is_owned p own = true)),
+    bmatch m b ofs p own (Tbox ty)
+| bm_struct: forall orgs id
+    (* all fields in the struct satisfy bmatch *)
+    (FMATCH: forall co fid fty fofs bf,
+        ce ! id = Some co ->
+        In (Member_plain fid fty) co.(co_members) ->       
+        field_offset ce fid co.(co_members) = OK (fofs, bf) ->
+        bmatch m b (ofs + fofs) (Pfield p fid fty) own fty),
+    bmatch m b ofs p own (Tstruct orgs id)
+| bm_enum: forall orgs id
+    (FMATCH: forall co fid fty fofs bf tag,
+        ce ! id = Some co ->
+        (* load tag *)
+        Mem.load Mint32 m b ofs = Some (Vint tag) ->
+        list_nth_z co.(co_members) (Int.unsigned tag) = Some (Member_plain fid fty) ->
+        variant_field_offset ce fid (co_members co) = OK (fofs, bf) ->        
+        bmatch m b (ofs + fofs) (Pdowncast p fid fty) own fty),
+    bmatch m b ofs p own (Tvariant orgs id)
+| bm_scalar: forall ty,
+    scalar_type ty = true ->
+    bmatch m b ofs p own ty
+(** TODO: bm_reference  *)
+.
+  
+
+Definition mmatch (m: mem) (own: own_env) : Prop :=
+  forall b ofs p pofs,
+    abs b ofs = Some (p, pofs) ->
+    (** TODO: how to represent the align_chunk property in
+    valid_access ? I think the permission depends on the type of p *)
+    (Mem.range_perm m b (ofs - pofs) (ofs - pofs + (sizeof ce (typeof_place p))) Cur Freeable
+    /\ bmatch m b (ofs - pofs) p own (typeof_place p)).
+
+
+End MATCH.
+
+
+
+Section BORCHK.
 
 Variable p: program.
 Variable w: inv_world wt_c.
@@ -20,11 +118,45 @@ Hypothesis INV: symtbl_inv wt_c w se.
 Let L := semantics p se.
 Let ge := globalenv se p.
 
-Variable sound_state: state -> Prop.
+(* composite environment *)
+Let ce := ge.(genv_cenv).
+
+
+Inductive sound_state: state -> Prop :=
+| sound_regular_state: forall
+    (CFG: generate_cfg f.(fn_body) = OK (entry, cfg))
+    (INSTR: cfg ! pc = Some instr)
+    (MSTMT: match_instr_stmt f.(fn_body) instr s k)
+    (CHK: borrow_check ce f = OK ae)
+    (AS: ae ! pc = Some (AE.State Σ Γ Δ))
+    
+    sound_state (State f s k e m)
+  
+
+  
 
 Lemma sound_state_no_mem_error: forall s,
     step_mem_error ge s -> sound_state s -> False .
 Admitted.
+
+Lemma initial_state_sound: forall q s,
+    Smallstep.initial_state L q s ->
+    sound_state s.
+Admitted.
+
+Lemma step_sound: forall s1 t s2,
+    sound_state s1 ->
+    Step L s1 t s2 ->
+    (* how to prove sound_state in dropstate? *)
+    sound_state s2.
+Admitted.
+
+
+Lemma reachable_state_sound: forall s,
+    (* What about after external? *)
+    reachable L s -> sound_state s.
+Admitted.
+
 
 (** Specific definition of partial safe *)
 Definition partial_safe (s: state) : Prop :=
@@ -37,14 +169,37 @@ Lemma borrow_check_lts_safe:
 Proof.
   intros BORCHK PSAFE. inv PSAFE.  
   constructor.
-  - simpl in *. intros s t s' STEP.
-    generalize (step_safe _ _ _ STEP). intros PSAFE.
+  - intros s t s' REACH STEP.
+    generalize (step_safe _ _ _ REACH STEP). intros PSAFE.
     destruct PSAFE as [|MEMERROR]. auto.
+    exfalso. eapply sound_state_no_mem_error. eauto.
+    eapply reachable_state_sound. eapply step_reachable; eauto.
+  (* initial_progress *)
+  - eauto.
+  (* initial_safe *)
+  - intros q s INIT.
+    generalize (initial_safe _ _ INIT). intros PSAFE.
+    destruct PSAFE as [|MEMERROR]. auto.
+    exfalso. eapply sound_state_no_mem_error. eauto.
+    eapply initial_state_sound; eauto.
+  (* external_safe *)
+  - intros s q REACH EXT.
+    generalize (external_safe _ _ REACH EXT).
+    intros (wA & SYMBINV & VQ & AFTEREXT).
+    exists wA. split; auto. split; auto.
+    intros r VR. generalize (AFTEREXT _ VR).
+    intros ((s' & AFTER) & PSAFE).
+    split. exists s'. eauto.
+    intros s'' AFTER1.
+    generalize (PSAFE s'' AFTER1). intros PSAFE1.
+    destruct PSAFE1 as [|MEMERROR]. auto.
+    exfalso. eapply sound_state_no_mem_error. eauto.
+    eapply reachable_state_sound. eapply external_reach; eauto.
+    eapply star_refl.
+  - eauto.
+Qed.    
     
-    
-Admitted.
-
-End BORROWCK.
+End BORCHK.
 
 
 
